LinearScan/Interval.hs
@@ -15,29 +15,48 @@ import qualified LinearScan.Range as Range
 __ :: any
 __ = Prelude.error "Logical or arity value used"
 
+data IntervalKind =
+   Whole
+ | LeftMost
+ | Middle
+ | RightMost
+
+splitKind :: IntervalKind -> (,) IntervalKind IntervalKind
+splitKind k =
+  case k of {
+   Whole -> (,) LeftMost RightMost;
+   LeftMost -> (,) LeftMost Middle;
+   Middle -> (,) Middle Middle;
+   RightMost -> (,) Middle RightMost}
+
 data IntervalDesc =
-   Build_IntervalDesc Prelude.Int Prelude.Int Prelude.Int ([]
-                                                          Range.RangeDesc)
+   Build_IntervalDesc Prelude.Int Prelude.Int Prelude.Int IntervalKind 
+ ([] Range.RangeDesc)
 
 ivar :: IntervalDesc -> Prelude.Int
 ivar i =
   case i of {
-   Build_IntervalDesc ivar0 ibeg0 iend0 rds0 -> ivar0}
+   Build_IntervalDesc ivar0 ibeg0 iend0 iknd0 rds0 -> ivar0}
 
 ibeg :: IntervalDesc -> Prelude.Int
 ibeg i =
   case i of {
-   Build_IntervalDesc ivar0 ibeg0 iend0 rds0 -> ibeg0}
+   Build_IntervalDesc ivar0 ibeg0 iend0 iknd0 rds0 -> ibeg0}
 
 iend :: IntervalDesc -> Prelude.Int
 iend i =
   case i of {
-   Build_IntervalDesc ivar0 ibeg0 iend0 rds0 -> iend0}
+   Build_IntervalDesc ivar0 ibeg0 iend0 iknd0 rds0 -> iend0}
+
+iknd :: IntervalDesc -> IntervalKind
+iknd i =
+  case i of {
+   Build_IntervalDesc ivar0 ibeg0 iend0 iknd0 rds0 -> iknd0}
 
 rds :: IntervalDesc -> [] Range.RangeDesc
 rds i =
   case i of {
-   Build_IntervalDesc ivar0 ibeg0 iend0 rds0 -> rds0}
+   Build_IntervalDesc ivar0 ibeg0 iend0 iknd0 rds0 -> rds0}
 
 getIntervalDesc :: IntervalDesc -> IntervalDesc
 getIntervalDesc d =
@@ -80,7 +99,7 @@ intervalIntersectionPoint i j =
 
 findIntervalUsePos :: IntervalDesc -> (Range.UsePos -> Prelude.Bool) ->
                       Prelude.Maybe ((,) Range.RangeDesc Range.UsePos)
-findIntervalUsePos i f =
+findIntervalUsePos d f =
   let {
    f0 = \r ->
     case Range.findRangeUsePos r f of {
@@ -95,13 +114,17 @@ findIntervalUsePos i f =
        (\r rs' ->
        Lib.option_choose (f0 r) (go rs'))
        rs}
-  in go (rds i)
+  in go (rds d)
 
 nextUseAfter :: IntervalDesc -> Prelude.Int -> Prelude.Maybe Prelude.Int
 nextUseAfter d pos =
   Lib.option_map ((Prelude..) Range.uloc Prelude.snd)
     (findIntervalUsePos d (\u ->
       (Prelude.<=) ((Prelude.succ) pos) (Range.uloc u)))
+
+firstUsePos :: IntervalDesc -> Prelude.Int
+firstUsePos d =
+  Range.uloc (Prelude.head (Range.ups ( (Prelude.head (rds d)))))
 
 firstUseReqReg :: IntervalDesc -> Prelude.Maybe Prelude.Int
 firstUseReqReg d =
@@ -117,262 +140,271 @@ splitPosition :: IntervalDesc -> SplitPosition -> Prelude.Maybe Prelude.Int
 splitPosition d pos =
   case pos of {
    BeforePos x -> Prelude.Just x;
-   BeforeFirstUsePosReqReg -> firstUseReqReg d;
+   BeforeFirstUsePosReqReg -> firstUseReqReg (getIntervalDesc d);
    EndOfLifetimeHole -> Prelude.Nothing}
 
 intervalSpan :: ([] Range.RangeDesc) -> Prelude.Int -> Prelude.Int ->
-                Prelude.Int -> Prelude.Int ->
+                Prelude.Int -> Prelude.Int -> IntervalKind ->
                 ((,) (Prelude.Maybe IntervalDesc)
                 (Prelude.Maybe IntervalDesc))
-intervalSpan rs before iv ib ie =
-  (\ns nc l -> case l of [x] -> ns x; (x:xs) -> nc x xs)
-    (\r ->
-    let {_top_assumption_ = Range.rangeSpan before ( r)} in
-    let {
-     _evar_0_ = \_top_assumption_0 ->
+intervalSpan rs before iv ib ie knd =
+  let {
+   _evar_0_ = \lknd rknd ->
+    (\ns nc l -> case l of [x] -> ns x; (x:xs) -> nc x xs)
+      (\r ->
+      let {_top_assumption_ = Range.rangeSpan before ( r)} in
       let {
-       _evar_0_ = \r0 _top_assumption_1 ->
+       _evar_0_ = \_top_assumption_0 ->
         let {
-         _evar_0_ = \r1 ->
+         _evar_0_ = \r0 _top_assumption_1 ->
           let {
-           _evar_0_ = let {
-                       _evar_0_ = \_ _ -> (,) (Prelude.Just
-                        (Build_IntervalDesc iv (Range.rbeg ( r0))
-                        (Range.rend ( r0)) ((:[]) ( r0)))) (Prelude.Just
-                        (Build_IntervalDesc iv (Range.rbeg ( r1))
-                        (Range.rend ( r1)) ((:[]) ( r1))))}
-                      in
-                       _evar_0_}
+           _evar_0_ = \r1 ->
+            let {
+             _evar_0_ = let {
+                         _evar_0_ = \_ _ -> (,) (Prelude.Just
+                          (Build_IntervalDesc iv (Range.rbeg ( r0))
+                          (Range.rend ( r0)) lknd ((:[]) ( r0))))
+                          (Prelude.Just (Build_IntervalDesc iv
+                          (Range.rbeg ( r1)) (Range.rend ( r1)) rknd ((:[])
+                          ( r1))))}
+                        in
+                         _evar_0_}
+            in
+             _evar_0_ __ __}
           in
-           _evar_0_ __ __}
-        in
-        let {
-         _evar_0_0 = let {
-                      _evar_0_0 = let {
-                                   _evar_0_0 = \_ -> (,) (Prelude.Just
-                                    (Build_IntervalDesc iv (Range.rbeg ( r0))
-                                    (Range.rend ( r0)) ((:[]) ( r0))))
-                                    Prelude.Nothing}
-                                  in
-                                   _evar_0_0}
-                     in
-                      _evar_0_0}
-        in
-        case _top_assumption_1 of {
-         Prelude.Just x -> (\_ -> _evar_0_ x);
-         Prelude.Nothing -> _evar_0_0}}
-      in
-      let {
-       _evar_0_0 = \_top_assumption_1 ->
-        let {
-         _evar_0_0 = \r1 ->
           let {
            _evar_0_0 = let {
-                        _evar_0_0 = \_ -> (,) Prelude.Nothing (Prelude.Just
-                         (Build_IntervalDesc iv (Range.rbeg ( r1))
-                         (Range.rend ( r1)) ((:[]) ( r1))))}
+                        _evar_0_0 = let {
+                                     _evar_0_0 = \_ -> (,) (Prelude.Just
+                                      (Build_IntervalDesc iv
+                                      (Range.rbeg ( r0)) (Range.rend ( r0))
+                                      knd ((:[]) ( r0)))) Prelude.Nothing}
+                                    in
+                                     _evar_0_0}
                        in
                         _evar_0_0}
           in
-           _evar_0_0}
-        in
-        let {_evar_0_1 = \_ -> Logic.coq_False_rec} in
-        case _top_assumption_1 of {
-         Prelude.Just x -> _evar_0_0 x;
-         Prelude.Nothing -> _evar_0_1}}
-      in
-      case _top_assumption_0 of {
-       Prelude.Just x -> _evar_0_ x;
-       Prelude.Nothing -> _evar_0_0}}
-    in
-    case _top_assumption_ of {
-     (,) x x0 -> _evar_0_ x x0 __})
-    (\r rs0 ->
-    let {_top_assumption_ = Range.rangeSpan before ( r)} in
-    let {
-     _evar_0_ = \_top_assumption_0 ->
-      let {
-       _evar_0_ = \r0 _top_assumption_1 ->
-        let {
-         _evar_0_ = \r1 ->
-          let {
-           _evar_0_ = \_ ->
-            (Prelude.flip (Prelude.$)) __ (\_ ->
-              let {
-               _evar_0_ = \_ -> (,) (Prelude.Just (Build_IntervalDesc iv
-                (Range.rbeg ( r0)) (Range.rend ( r0)) ((:[]) ( r0))))
-                (Prelude.Just (Build_IntervalDesc iv (Range.rbeg ( r1))
-                (Range.rend ( (Prelude.last rs0))) ((:) r1 rs0)))}
-              in
-               _evar_0_ __)}
-          in
-           _evar_0_ __}
+          case _top_assumption_1 of {
+           Prelude.Just x -> (\_ -> _evar_0_ x);
+           Prelude.Nothing -> _evar_0_0}}
         in
         let {
-         _evar_0_0 = \_ ->
+         _evar_0_0 = \_top_assumption_1 ->
           let {
-           _evar_0_0 = \_ ->
+           _evar_0_0 = \r1 ->
             let {
-             _top_assumption_2 = intervalSpan rs0 before iv
-                                   (Range.rbeg ( (Prelude.head rs0)))
-                                   (Range.rend ( (Prelude.last rs0)))}
+             _evar_0_0 = let {
+                          _evar_0_0 = \_ -> (,) Prelude.Nothing (Prelude.Just
+                           (Build_IntervalDesc iv (Range.rbeg ( r1))
+                           (Range.rend ( r1)) knd ((:[]) ( r1))))}
+                         in
+                          _evar_0_0}
             in
-            let {
-             _evar_0_0 = \_top_assumption_3 ->
-              let {
-               _evar_0_0 = \i1_1 _top_assumption_4 ->
-                let {
-                 _evar_0_0 = \i1_2 ->
-                  case i1_1 of {
-                   Build_IntervalDesc ivar0 ibeg0 iend0 rds0 ->
-                    let {
-                     _evar_0_0 = let {
-                                  _evar_0_0 = \_ ->
-                                   let {
-                                    _evar_0_0 = \_ ->
-                                     let {
-                                      _evar_0_0 = \_ ->
-                                       (Prelude.flip (Prelude.$)) __ (\_ ->
-                                         let {
-                                          _evar_0_0 = let {
-                                                       _evar_0_0 = \_ _ _ ->
-                                                        (,) (Prelude.Just
-                                                        (Build_IntervalDesc
-                                                        ivar0
-                                                        (Range.rbeg ( r))
-                                                        iend0 ((:) r rds0)))
-                                                        (Prelude.Just i1_2)}
-                                                      in
-                                                       _evar_0_0 __}
-                                         in
-                                          _evar_0_0)}
-                                     in
-                                      _evar_0_0 __}
-                                   in
-                                    _evar_0_0 __}
-                                 in
-                                  _evar_0_0}
-                    in
-                     _evar_0_0 __}}
-                in
-                let {
-                 _evar_0_1 = \_ _ _ ->
-                  case i1_1 of {
-                   Build_IntervalDesc ivar0 ibeg0 iend0 rds0 ->
-                    let {
-                     _evar_0_1 = let {
-                                  _evar_0_1 = \_ ->
-                                   (Prelude.flip (Prelude.$)) __ (\_ ->
-                                     (Prelude.flip (Prelude.$)) __ (\_ ->
-                                       let {
-                                        _evar_0_1 = \_ ->
-                                         let {
-                                          _evar_0_1 = \_ -> (,) (Prelude.Just
-                                           (Build_IntervalDesc ivar0
-                                           (Range.rbeg ( r)) iend0 ((:) r
-                                           rds0))) Prelude.Nothing}
-                                         in
-                                          _evar_0_1 __}
-                                       in
-                                        _evar_0_1 __))}
-                                 in
-                                  _evar_0_1}
-                    in
-                     _evar_0_1 __}}
-                in
-                case _top_assumption_4 of {
-                 Prelude.Just x -> (\_ -> _evar_0_0 x);
-                 Prelude.Nothing -> _evar_0_1}}
-              in
-              let {
-               _evar_0_1 = \_top_assumption_4 ->
-                let {
-                 _evar_0_1 = \i1_2 ->
-                  case i1_2 of {
-                   Build_IntervalDesc ivar0 ibeg0 iend0 rds0 ->
-                    let {
-                     _evar_0_1 = let {
-                                  _evar_0_1 = \_ ->
-                                   let {
-                                    _evar_0_1 = \_ _ ->
-                                     let {
-                                      _evar_0_1 = \_ ->
-                                       let {
-                                        _evar_0_1 = \_ ->
-                                         let {
-                                          _evar_0_1 = \_ ->
-                                           (Prelude.flip (Prelude.$)) __
-                                             (\_ -> (,) (Prelude.Just
-                                             (Build_IntervalDesc iv
-                                             (Range.rbeg ( r0))
-                                             (Range.rend ( r0)) ((:[])
-                                             ( r0)))) (Prelude.Just
-                                             (Build_IntervalDesc ivar0
-                                             (Range.rbeg
-                                               ( (Prelude.head rds0)))
-                                             (Range.rend
-                                               ( (Prelude.last rds0)))
-                                             rds0)))}
-                                         in
-                                          _evar_0_1 __}
-                                       in
-                                        _evar_0_1 __}
-                                     in
-                                      _evar_0_1 __}
-                                   in
-                                    _evar_0_1 __ __}
-                                 in
-                                  _evar_0_1}
-                    in
-                     _evar_0_1 __}}
-                in
-                let {_evar_0_2 = \_ _ _ -> Logic.coq_False_rec} in
-                case _top_assumption_4 of {
-                 Prelude.Just x -> (\_ _ _ -> _evar_0_1 x);
-                 Prelude.Nothing -> _evar_0_2}}
-              in
-              case _top_assumption_3 of {
-               Prelude.Just x -> _evar_0_0 x;
-               Prelude.Nothing -> _evar_0_1}}
-            in
-            case _top_assumption_2 of {
-             (,) x x0 -> _evar_0_0 x x0 __ __ __}}
+             _evar_0_0}
           in
-           _evar_0_0 __}
+          let {_evar_0_1 = \_ -> Logic.coq_False_rec} in
+          case _top_assumption_1 of {
+           Prelude.Just x -> _evar_0_0 x;
+           Prelude.Nothing -> _evar_0_1}}
         in
-        case _top_assumption_1 of {
-         Prelude.Just x -> (\_ -> _evar_0_ x);
+        case _top_assumption_0 of {
+         Prelude.Just x -> _evar_0_ x;
          Prelude.Nothing -> _evar_0_0}}
       in
+      case _top_assumption_ of {
+       (,) x x0 -> _evar_0_ x x0 __})
+      (\r rs0 ->
+      let {_top_assumption_ = Range.rangeSpan before ( r)} in
       let {
-       _evar_0_0 = \_top_assumption_1 ->
+       _evar_0_ = \_top_assumption_0 ->
         let {
-         _evar_0_0 = \r1 ->
+         _evar_0_ = \r0 _top_assumption_1 ->
+          let {
+           _evar_0_ = \r1 ->
+            let {
+             _evar_0_ = \_ ->
+              (Prelude.flip (Prelude.$)) __ (\_ ->
+                let {
+                 _evar_0_ = \_ -> (,) (Prelude.Just (Build_IntervalDesc iv
+                  (Range.rbeg ( r0)) (Range.rend ( r0)) lknd ((:[]) ( r0))))
+                  (Prelude.Just (Build_IntervalDesc iv (Range.rbeg ( r1))
+                  (Range.rend ( (Prelude.last rs0))) knd ((:) r1 rs0)))}
+                in
+                 _evar_0_ __)}
+            in
+             _evar_0_ __}
+          in
           let {
            _evar_0_0 = \_ ->
             let {
              _evar_0_0 = \_ ->
               let {
-               _evar_0_0 = \_ -> (,) Prelude.Nothing (Prelude.Just
-                (Build_IntervalDesc iv (Range.rbeg ( r1))
-                (Range.rend ( (Prelude.last rs0))) ((:) r1 rs0)))}
+               _top_assumption_2 = intervalSpan rs0 before iv
+                                     (Range.rbeg ( (Prelude.head rs0)))
+                                     (Range.rend ( (Prelude.last rs0))) knd}
+              in
+              let {
+               _evar_0_0 = \_top_assumption_3 ->
+                let {
+                 _evar_0_0 = \i1_1 _top_assumption_4 ->
+                  let {
+                   _evar_0_0 = \i1_2 ->
+                    case i1_1 of {
+                     Build_IntervalDesc ivar0 ibeg0 iend0 iknd0 rds0 ->
+                      let {
+                       _evar_0_0 = let {
+                                    _evar_0_0 = \_ ->
+                                     let {
+                                      _evar_0_0 = \_ ->
+                                       let {
+                                        _evar_0_0 = \_ ->
+                                         (Prelude.flip (Prelude.$)) __ (\_ ->
+                                           let {
+                                            _evar_0_0 = let {
+                                                         _evar_0_0 = \_ _ _ ->
+                                                          (,) (Prelude.Just
+                                                          (Build_IntervalDesc
+                                                          ivar0
+                                                          (Range.rbeg ( r))
+                                                          iend0 iknd0 ((:) r
+                                                          rds0)))
+                                                          (Prelude.Just
+                                                          i1_2)}
+                                                        in
+                                                         _evar_0_0 __}
+                                           in
+                                            _evar_0_0)}
+                                       in
+                                        _evar_0_0 __}
+                                     in
+                                      _evar_0_0 __}
+                                   in
+                                    _evar_0_0}
+                      in
+                       _evar_0_0 __}}
+                  in
+                  let {
+                   _evar_0_1 = \_ _ _ ->
+                    case i1_1 of {
+                     Build_IntervalDesc ivar0 ibeg0 iend0 iknd0 rds0 ->
+                      let {
+                       _evar_0_1 = let {
+                                    _evar_0_1 = \_ ->
+                                     (Prelude.flip (Prelude.$)) __ (\_ ->
+                                       (Prelude.flip (Prelude.$)) __ (\_ ->
+                                         let {
+                                          _evar_0_1 = \_ ->
+                                           let {
+                                            _evar_0_1 = \_ -> (,)
+                                             (Prelude.Just
+                                             (Build_IntervalDesc ivar0
+                                             (Range.rbeg ( r)) iend0 iknd0
+                                             ((:) r rds0))) Prelude.Nothing}
+                                           in
+                                            _evar_0_1 __}
+                                         in
+                                          _evar_0_1 __))}
+                                   in
+                                    _evar_0_1}
+                      in
+                       _evar_0_1 __}}
+                  in
+                  case _top_assumption_4 of {
+                   Prelude.Just x -> (\_ -> _evar_0_0 x);
+                   Prelude.Nothing -> _evar_0_1}}
+                in
+                let {
+                 _evar_0_1 = \_top_assumption_4 ->
+                  let {
+                   _evar_0_1 = \i1_2 ->
+                    case i1_2 of {
+                     Build_IntervalDesc ivar0 ibeg0 iend0 iknd0 rds0 ->
+                      let {
+                       _evar_0_1 = let {
+                                    _evar_0_1 = \_ ->
+                                     let {
+                                      _evar_0_1 = \_ _ ->
+                                       let {
+                                        _evar_0_1 = \_ ->
+                                         let {
+                                          _evar_0_1 = \_ ->
+                                           let {
+                                            _evar_0_1 = \_ ->
+                                             (Prelude.flip (Prelude.$)) __
+                                               (\_ -> (,) (Prelude.Just
+                                               (Build_IntervalDesc iv
+                                               (Range.rbeg ( r0))
+                                               (Range.rend ( r0)) lknd ((:[])
+                                               ( r0)))) (Prelude.Just
+                                               (Build_IntervalDesc ivar0
+                                               (Range.rbeg
+                                                 ( (Prelude.head rds0)))
+                                               (Range.rend
+                                                 ( (Prelude.last rds0)))
+                                               iknd0 rds0)))}
+                                           in
+                                            _evar_0_1 __}
+                                         in
+                                          _evar_0_1 __}
+                                       in
+                                        _evar_0_1 __}
+                                     in
+                                      _evar_0_1 __ __}
+                                   in
+                                    _evar_0_1}
+                      in
+                       _evar_0_1 __}}
+                  in
+                  let {_evar_0_2 = \_ _ _ -> Logic.coq_False_rec} in
+                  case _top_assumption_4 of {
+                   Prelude.Just x -> (\_ _ _ -> _evar_0_1 x);
+                   Prelude.Nothing -> _evar_0_2}}
+                in
+                case _top_assumption_3 of {
+                 Prelude.Just x -> _evar_0_0 x;
+                 Prelude.Nothing -> _evar_0_1}}
+              in
+              case _top_assumption_2 of {
+               (,) x x0 -> _evar_0_0 x x0 __ __ __}}
+            in
+             _evar_0_0 __}
+          in
+          case _top_assumption_1 of {
+           Prelude.Just x -> (\_ -> _evar_0_ x);
+           Prelude.Nothing -> _evar_0_0}}
+        in
+        let {
+         _evar_0_0 = \_top_assumption_1 ->
+          let {
+           _evar_0_0 = \r1 ->
+            let {
+             _evar_0_0 = \_ ->
+              let {
+               _evar_0_0 = \_ ->
+                let {
+                 _evar_0_0 = \_ -> (,) Prelude.Nothing (Prelude.Just
+                  (Build_IntervalDesc iv (Range.rbeg ( r1))
+                  (Range.rend ( (Prelude.last rs0))) knd ((:) r1 rs0)))}
+                in
+                 _evar_0_0 __}
               in
                _evar_0_0 __}
             in
              _evar_0_0 __}
           in
-           _evar_0_0 __}
+          let {_evar_0_1 = \_ -> Logic.coq_False_rec} in
+          case _top_assumption_1 of {
+           Prelude.Just x -> (\_ -> _evar_0_0 x);
+           Prelude.Nothing -> _evar_0_1}}
         in
-        let {_evar_0_1 = \_ -> Logic.coq_False_rec} in
-        case _top_assumption_1 of {
-         Prelude.Just x -> (\_ -> _evar_0_0 x);
-         Prelude.Nothing -> _evar_0_1}}
+        case _top_assumption_0 of {
+         Prelude.Just x -> _evar_0_ x;
+         Prelude.Nothing -> _evar_0_0}}
       in
-      case _top_assumption_0 of {
-       Prelude.Just x -> _evar_0_ x;
-       Prelude.Nothing -> _evar_0_0}}
-    in
-    case _top_assumption_ of {
-     (,) x x0 -> _evar_0_ x x0 __})
-    rs
+      case _top_assumption_ of {
+       (,) x x0 -> _evar_0_ x x0 __})
+      rs}
+  in
+  case splitKind knd of {
+   (,) x x0 -> _evar_0_ x x0}
 
